working on generating ModWf proofs

example/out/ProcDecExec.v
@@ -130,8 +130,12 @@ Module module'mkDecExec.
         Retv ) (* rule decexecToHost *)
     }). (* mkDecExec *)
 
+    Hint Unfold mkDecExecModule : ModuleDefs.
+    Definition wellformed_mkDecExecModule : ModWf := @Build_ModWf mkDecExecModule ltac:(intros; repeat autounfold with ModuleDefs; discharge_wf).
+
 (* Module mkDecExec type RegFile#(Bit#(PgmSz), Bit#(InstrSz)) -> Decoder -> Executer -> Scoreboard -> FIFO#(E2W) -> ProcRegs -> Memory -> ToHost -> Module#(Empty) return type Decoder *)
     Definition mkDecExec := Build_Empty mkDecExecModule%kami.
+    Hint Unfold mkDecExec : ModuleDefs.
     End Section'mkDecExec.
 End module'mkDecExec.
 
@@ -139,6 +143,23 @@ Definition mkDecExec := module'mkDecExec.mkDecExec.
 Hint Unfold mkDecExec : ModuleDefs.
 Hint Unfold module'mkDecExec.mkDecExec : ModuleDefs.
 Hint Unfold module'mkDecExec.mkDecExecModule : ModuleDefs.
+
+Theorem wellformed_mkDecExecModule:
+  forall prefix: string,
+  forall rf: RegFile,
+  forall dec : Decoder,
+  forall exec: Executer,
+  forall sc: Scoreboard,
+  forall fifo: FIFO,
+  forall regs: ProcRegs,
+  forall mem: Memory,
+  forall th: ToHost,
+  WfMod (module'mkDecExec.mkDecExecModule prefix rf dec exec sc fifo regs mem th).
+Proof.
+  intros.
+  repeat autounfold with ModuleDefs.
+  discharge_wf.
+Qed.
 
 Module module'mkDecExecSep.
     Section Section'mkDecExecSep.
